fsub/lngen/prop_basic.v
@@ -1,2 +1,27 @@
+Require Import Coq.Program.Equality.
+Require Import Metalib.Metatheory.
+From Hammer Require Import Tactics.
+
 Require Import fsub.lngen.def_ott.
 Require Import fsub.lngen.prop_ln.
+Require Import common.ltac_ln.
+Require Import common.prop_ln.
+Require Import fsub.lngen.def_extra.
+
+Lemma wf_typ_lc_typ Γ A :
+  Γ ⊢ A -> 
+  lc_typ A.
+Proof.
+  intros. induction H; try hauto ctrs:lc_typ.
+  - pick fresh X. inst_cofinites_with X.
+    eapply lc_typ_all_exists with X; eauto.
+Qed.
+
+Lemma subtyping_lc_typ Γ A B :
+  Γ ⊢ A <: B -> 
+  lc_typ A /\ lc_typ B.
+Proof.
+  intros. induction H; try hauto ctrs:lc_typ use:wf_typ_lc_typ.
+  - split; pick fresh X; inst_cofinites_with X; 
+    eapply lc_typ_all_exists with X; hauto.
+Qed.
